Lean4Lean/Theory.lean
@@ -4,3 +4,5 @@ import Lean4Lean.Theory.Typing.Strong
 import Lean4Lean.Theory.Typing.UniqueTyping
 import Lean4Lean.Theory.Typing.ChurchRosser
 import Lean4Lean.Theory.Typing.HeadReduction
+import Lean4Lean.Theory.LocalContext
+import Lean4Lean.Theory.Literals
